theories/iris_examples.v
@@ -1,0 +1,280 @@
+From mathcomp Require Import ssreflect eqtype seq ssrbool.
+From iris.program_logic Require Import language.
+From iris.proofmode Require Import tactics.
+From iris.program_logic Require Export weakestpre lifting.
+From iris.base_logic Require Export gen_heap proph_map.
+Require Export iris iris_locations iris_properties iris_atomicity stdpp_aux.
+Require Export iris_use.
+Require Export datatypes host operations properties opsem.
+
+Set Implicit Arguments.
+Unset Strict Implicit.
+Unset Printing Implicit Defensive.
+
+Close Scope byte_scope.
+
+Let expr := iris.expr.
+Let val := iris.val.
+Let to_val := iris.to_val.
+
+(* Example Programs *)
+Section Examples.
+
+Context `{!wfuncG host_function Σ, !wtabG Σ, !wmemG Σ, !wmemsizeG Σ, !wglobG Σ, !wlocsG Σ, !winstG Σ(*, irisG (wasm_lang host_function host_instance) Σ*)}.
+
+Let host := host.host host_function.
+Let function_closure := function_closure host_function.
+Let store_record := store_record host_function.
+
+Variable host_instance: host.
+
+Let reduce := @reduce host_function host_instance.
+
+
+(*
+Let wasm_mixin : LanguageMixin _ _ _ := wasm_mixin host_instance.
+
+Canonical Structure wasm_lang := Language wasm_mixin.
+
+Let reducible := @reducible wasm_lang.
+
+Let prim_step := @iris.prim_step host_function host_instance.
+*)
+
+Definition xx i := (VAL_int32 (Wasm_int.int_of_Z i32m i)).
+Definition xb b := (VAL_int32 (wasm_bool b)).
+
+Definition my_add : expr :=
+  [AI_basic (BI_const (xx 3));
+     AI_basic (BI_const (xx 2));
+  AI_basic (BI_binop T_i32 (Binop_i BOI_add))].
+
+(* Doesn't work yet -- there are some typeclass and context bugs to be fixed *)
+Lemma myadd_spec (s : stuckness) (E : coPset) (Φ: val -> iProp Σ) : 
+  Φ (immV [xx 5]) ⊢ WP my_add @ s; E {{ v, Φ v }}.
+Proof.
+  iIntros "HΦ".
+  unfold my_add.
+  by iApply wp_binop.
+Qed.
+
+(* An example to show framing from the stack. *)
+Definition my_add2: expr :=
+  [AI_basic (BI_const (xx 1));
+  AI_basic (BI_const (xx 2));
+  AI_basic (BI_binop T_i32 (Binop_i BOI_add));
+  AI_basic (BI_const (xx 2));
+  AI_basic (BI_binop T_i32 (Binop_i BOI_add))].
+
+Lemma myadd2_spec (s : stuckness) (E : coPset) (Φ: val -> iProp Σ) :
+  Φ (immV [xx 5]) ⊢ WP my_add2 @ s; E {{ v, Φ v }}.
+Proof.
+  iIntros "HΦ".
+  replace my_add2 with (take 3 my_add2 ++ drop 3 my_add2) => //.
+  iApply wp_seq => /=.
+  instantiate (1 := fun v => (⌜ v = immV [xx 3] ⌝)%I ).
+  iSplit => //.
+  iSplitR "HΦ"; first by iApply wp_binop.
+  iIntros (? ->) => /=.
+  by iApply wp_binop.
+Qed.
+
+(* --------------------------------------------------------------------------------------------- *)
+(* -------------------------------- CONTROL FLOW EXAMPLES -------------------------------------- *)
+(* --------------------------------------------------------------------------------------------- *)
+
+(* Helper lemmas and tactics for necessary list manipulations for expressions *)
+Lemma iRewrite_nil_l (s : stuckness) (E : coPset) (Φ : val -> iProp Σ) (e : iris.expr) :
+  (WP [] ++ e @ s; E {{ Φ }} ⊢ WP e @ s; E {{ Φ }}).
+Proof. rewrite app_nil_l. auto. Qed.
+Lemma iRewrite_nil_r (s : stuckness) (E : coPset) (Φ : val -> iProp Σ) (e : iris.expr) :
+  (WP e ++ [] @ s; E {{ Φ }} ⊢ WP e @ s; E {{ Φ }}).
+Proof. rewrite app_nil_r. auto. Qed.
+Lemma iRewrite_nil_l_ctx (s : stuckness) (E : coPset) (Φ : val -> iProp Σ) (e : iris.expr) i lh :
+  (WP [] ++ e @ s; E CTX i; lh {{ Φ }} ⊢ WP e @ s; E CTX i; lh {{ Φ }}).
+Proof. rewrite app_nil_l. auto. Qed.
+Lemma iRewrite_nil_r_ctx (s : stuckness) (E : coPset) (Φ : val -> iProp Σ) (e : iris.expr) i lh :
+  (WP e ++ [] @ s; E CTX i; lh {{ Φ }} ⊢ WP e @ s; E CTX i; lh {{ Φ }}).
+Proof. rewrite app_nil_r. auto. Qed.
+
+Ltac take_drop_app_rewrite n :=
+  match goal with
+  | |- context [ WP ?e @ _; _ CTX _; _ {{ _ }} %I ] =>
+      rewrite -(take_drop n e);simpl take; simpl drop
+  | |- context [ WP ?e @ _; _ {{ _ }} %I ] =>
+      rewrite -(take_drop n e);simpl take; simpl drop
+  end.
+
+Ltac take_drop_app_rewrite_twice n m :=
+  take_drop_app_rewrite n;
+  match goal with
+  | |- context [ WP _ ++ ?e @ _; _ CTX _; _ {{ _ }} %I ] =>
+      rewrite -(take_drop (length e - m) e);simpl take; simpl drop
+  | |- context [ WP _ ++ ?e @ _; _ {{ _ }} %I ] =>
+      rewrite -(take_drop (length e - m) e);simpl take; simpl drop
+  end.
+
+(* Examples of blocks that return normally *)
+Lemma label_check_easy :
+  ⊢ WP [::AI_basic
+         (BI_block (Tf [] [T_i32;T_i32])
+            [::BI_const (xx 2); BI_const (xx 3)] )] {{ λ v, ⌜v = immV [xx 2;xx 3]⌝ }}.
+Proof.
+  rewrite -iRewrite_nil_l.
+  iApply wp_block;eauto. iNext.
+  iApply wp_wasm_empty_ctx.
+  iApply wp_label_push_nil. simpl.
+  iApply wp_val_return;auto.
+  iApply wp_value;eauto. done.
+Qed.
+Lemma label_check_easy' :
+  ⊢ WP [::AI_basic
+         (BI_block (Tf [] [T_i32;T_i32])
+                   [:: (BI_block (Tf [] [T_i32;T_i32])
+                                [::BI_const (xx 2); BI_const (xx 3)] )] )] {{ λ v, ⌜v = immV [xx 2;xx 3]⌝ }}.
+Proof.
+  rewrite -iRewrite_nil_l.
+  iApply wp_block;eauto. iNext.
+  iApply wp_wasm_empty_ctx.
+  iApply wp_label_push_nil. simpl.
+  iApply iRewrite_nil_r_ctx.
+  iApply (wp_seq_ctx _ _ _ (λ v, ⌜v = immV [xx 2; xx 3]⌝)%I).
+  iSplitR.
+  iApply label_check_easy.
+  iIntros (w ->). simpl.
+  iApply wp_val_return;auto.
+  iApply wp_value;eauto. done.
+Qed.
+
+Lemma br_check_bind_return :
+  ⊢ WP [::AI_basic
+         (BI_block (Tf [] [T_i32])
+         [:: BI_block (Tf [] [])
+            [::BI_const (xx 3); BI_br 1] ])] {{ λ v, ⌜v = immV [xx 3]⌝ }}.
+Proof.
+  iApply iRewrite_nil_l.
+  iApply wp_block;eauto. iNext.
+  simpl.
+  iApply wp_wasm_empty_ctx.
+  iApply wp_label_push_nil.
+  simpl.
+  iApply iRewrite_nil_l_ctx.
+  iApply wp_block_ctx;eauto. iNext.
+  simpl.
+  iApply wp_label_push_nil.
+  simpl.
+  take_drop_app_rewrite 1.
+  iApply wp_br_ctx;auto. iNext.
+  iApply wp_value;auto. done.
+Qed.
+
+Lemma br_check_bind_return_2 :
+  ⊢ WP [::AI_basic
+         (BI_block (Tf [] [T_i32])
+         [:: BI_block (Tf [] [])
+            [::BI_const (xx 2);BI_const (xx 3); BI_br 1] ])] {{ λ v, ⌜v = immV [xx 3]⌝ }}.
+Proof.
+  iApply iRewrite_nil_l.
+  iApply wp_block;eauto. iNext.
+  simpl.
+  iApply wp_wasm_empty_ctx.
+  iApply wp_label_push_nil.
+  simpl.
+  iApply iRewrite_nil_l_ctx.
+  iApply wp_block_ctx;eauto. iNext.
+  simpl.
+  iApply wp_label_push_nil.
+  simpl.
+  take_drop_app_rewrite 1.
+  iApply iRewrite_nil_r_ctx.
+  rewrite -app_assoc.
+  iApply wp_base_push;auto.
+  take_drop_app_rewrite 1.
+  iApply wp_br_ctx;auto. iNext.
+  iApply wp_value;auto. done.
+Qed.
+
+Lemma br_check_bind_return_3 :
+  ⊢ WP [::AI_basic
+         (BI_block (Tf [] [T_i32])
+         [:: BI_block (Tf [] [])
+            [::BI_const (xx 2); BI_const (xx 3); (BI_binop T_i32 (Binop_i BOI_add)); BI_br 1] ])] {{ λ v, ⌜v = immV [xx 5]⌝ }}.
+Proof.
+  iApply iRewrite_nil_l.
+  iApply wp_block;eauto. iNext. simpl.
+  iApply wp_wasm_empty_ctx.
+  iApply wp_label_push_nil.
+  iApply iRewrite_nil_l_ctx.
+  iApply wp_block_ctx;eauto;simpl.
+  iApply wp_label_push_nil. iNext. simpl.
+  take_drop_app_rewrite 3.
+  iApply (wp_seq_ctx _ _ _ (λ v, ⌜v = immV [xx 5]⌝)%I).
+  iSplitR.
+  { iApply wp_binop;eauto. }
+  iIntros (w ->). simpl.
+  take_drop_app_rewrite 1.
+  iApply iRewrite_nil_l_ctx.
+  iApply iRewrite_nil_r_ctx. rewrite -!app_assoc.
+  iApply wp_br_ctx;auto. iNext. simpl.
+  iApply wp_value;eauto. done.  
+Qed.
+
+Lemma br_check_bind_return_4 :
+  ⊢ WP [::AI_basic
+         (BI_block (Tf [] [T_i32]) (* this block returns normally *)
+                   [:: BI_const (xx 1);
+                    BI_block (Tf [] [T_i32]) (* this block gets br'ed to *)
+                             [::BI_block (Tf [] []) (* this block will never return *)
+                               [::BI_const (xx 2);
+                                BI_const (xx 3);
+                                (BI_binop T_i32 (Binop_i BOI_add));
+                                BI_br 1;
+                                (BI_binop T_i32 (Binop_i BOI_add))] (* this expression gets stuck without br *) ];
+                    (BI_binop T_i32 (Binop_i BOI_add)) ])] (* this expression only reds after previous block is reduced *)
+    {{ λ v, ⌜v = immV [xx 6]⌝ }}.
+Proof.
+  iApply iRewrite_nil_l.
+  iApply wp_block;eauto. iNext. simpl.
+  iApply wp_wasm_empty_ctx.
+  iApply wp_label_push_nil. simpl.
+  iApply iRewrite_nil_r_ctx.
+  iApply (wp_seq_ctx _ _ _ (λ v, ⌜v = immV [xx 6]⌝)%I).
+  iSplitR.
+  { take_drop_app_rewrite_twice 1 1.
+    iApply wp_wasm_empty_ctx.
+    iApply wp_base_push;auto. simpl.
+    iApply iRewrite_nil_r_ctx.
+    iApply (wp_seq_ctx _ _ _ (λ v, ⌜v = immV [xx 5]⌝)%I).
+    iSplitR.
+    { iApply iRewrite_nil_l.
+      iApply wp_block;eauto. iNext. simpl.
+      iApply wp_wasm_empty_ctx.
+      iApply wp_label_push_nil. simpl.
+      iApply iRewrite_nil_l_ctx.
+      iApply wp_block_ctx;eauto. simpl. iNext.
+      iApply wp_label_push_nil. simpl.
+      take_drop_app_rewrite 3.
+      iApply (wp_seq_ctx _ _ _ (λ v, ⌜v = immV [xx 5]⌝)%I).
+      iSplitR.
+      { iApply wp_binop;eauto. }
+      iIntros (w ->). simpl.
+      take_drop_app_rewrite 2.
+      iApply iRewrite_nil_l_ctx.
+      iApply wp_base_push;auto. simpl.
+      take_drop_app_rewrite 1.
+      iApply wp_br_ctx;auto. iNext.
+      iApply wp_value;eauto. done. }
+    iIntros (w ->). simpl.
+    iApply wp_base;auto. simpl.
+    iApply wp_binop;eauto. }
+  iIntros (w ->) "/=".
+  iApply wp_val_return;auto;simpl.
+  iApply wp_value;eauto. done.
+Qed.
+  
+
+(* --------------------------------------------------------------------------------------------- *)
+(* --------------------------------- END OF EXAMPLES ------------------------------------------- *)
+(* --------------------------------------------------------------------------------------------- *)
+
+End Examples.
